chore

Auto/Embedding/Lift.lean
@@ -16,7 +16,7 @@ def orLift.{u} (p q : GLift.{1, u} Prop) :=
 def iffLift.{u} (p q : GLift.{1, u} Prop) :=
   GLift.up (Iff p.down q.down)
 
-def impF.{u, v} (p : Sort u) (q : Sort v) := p → q
+def ImpF.{u, v} (p : Sort u) (q : Sort v) := p → q
 
 def impLift.{u}
   (p : GLift.{t + 1, v} (Sort t))
